Makefile
@@ -6,46 +6,15 @@ coq: Makefile.coq
 Makefile.coq: Makefile.source
 	coq_makefile -f Makefile.source -o Makefile.coq
 
-doc:
+gen-html:
 	$(MAKE) -f Makefile.coq html COQDOCFLAGS="-interpolate -utf8 -g"
+
+gen-tex:
+	$(MAKE) -f Makefile.coq latex
 
 clean:
 	rm -f */*.vo */*.v.d */*.glob */*~ */.#* Makefile.coq
 	rm -f */*/*.vo */*/*.v.d */*/*.glob
-
-test: coq
-	$(MAKE) -C sealing runtest
-
-SHARED=lib/*.v common/*.v concrete/*.v symbolic/*.v
-
-SPECIF=memory_safety/*.v sealing/*.v compartmentalization/*.v cfi/*.v
-
-bc:
-	@echo "The shared/common/framework part"
-	@echo "     spec    proof comments"
-	@coqwc $(SHARED) | grep total
-	@echo "The policy-specific parts"
-	@echo "     spec    proof comments"
-	@coqwc $(SPECIF) | grep total
-	@echo "The total"
-	@echo "     spec    proof comments"
-	@coqwc $(SHARED) $(SPECIF) | grep total
-
-dist: clean
-	rm -f rm ../micropolicies.tar.gz
-	tar czvf ../micropolicies.tar.gz . --transform 's/^\./micropolicies/' --exclude=testing --exclude=.gitignore --exclude=cfi/review.org --exclude=compartmentalization/global-hint.el
-
-DIR=../micropolicies-coq-anon
-
-dist-anon: clean
-	rm -dfr rm $(DIR) ../micropolicies-coq-anon.tar.gz
-	cp -R . $(DIR)
-	rm -dfr $(DIR)/.git
-	perl -0777 -i -pe 's/Copyright.*Permission/Copyright Anonymized\n\nPermission/igs' $(DIR)/LICENSE
-	perl -0777 -i -pe 's/Description.*Prerequisites/Prerequisites/igs' $(DIR)/README.md
-        # Next command doesn't work for nested comments, please don't add any until Saturday
-	find $(DIR) -name '*.v' -exec perl -0777 -i -pe 's/\(\*.*?\*\)//igs' {} \;
-	cd $(DIR); tar czvf ../micropolicies-coq-anon.tar.gz . --transform 's/^\./micropolicies-coq-anon/' --exclude=testing --exclude=.gitignore --exclude=cfi/review.org --exclude=compartmentalization/global-hint.el
 
 coqide:
 	coqide -R . Brenner
